restore the previous trace_inv/trace_is setup, which was good, actually refactor the definition of linearizability to make it easier to handle and finish proving the adequacy for linearizability.v

theories/heap_lang/adequacy.v
@@ -30,61 +30,63 @@ Proof.
   iFrame. iApply (Hwp (HeapG _ _ _ _ _)).
 Qed.
 
-Definition heap_invariance Σ `{!heapPreG Σ} (N: namespace) (I: iProp Σ) (φ : list val → Prop) s e σ tp σ' :
-  (∀ `{!heapG Σ},
-    (⊢ trace_is (trace σ) ==∗ inv N I) ∧
-    (⊢ inv N I -∗ WP e @ s; ⊤ {{ _, True }}) ∧
-    (⊢ trace_auth (trace σ') -∗ ▷ I -∗ ⌜φ (trace σ')⌝)) →
-  rtc erased_step ([e], σ) (tp, σ') →
-  φ (trace σ').
+Definition heap_invariance Σ `{!heapPreG Σ} (N: namespace) (I: list val → Prop) s e σ :
+  I (trace σ) →
+  (∀ `{!heapG Σ}, ⊢ trace_inv N I -∗ trace_is (trace σ) -∗ WP e @ s; ⊤ {{ _, True }}) →
+  ∀ σ' t,
+    rtc erased_step ([e], σ) (t, σ') →
+    I (trace σ').
 Proof.
-  intros HI.
-  eapply (wp_invariance Σ _ s _ _ _ _ (φ (trace σ'))). iIntros (Hinv κs) "".
+  intros HI Hwp σ' t.
+  eapply (wp_invariance Σ _ s _ _ _ _ (I (trace σ'))). iIntros (Hinv κs) "".
   iMod (gen_heap_init σ.(heap)) as (?) "Hh".
   iMod (proph_map_init κs σ.(used_proph_id)) as (?) "Hp".
   iMod (trace_auth_init σ.(trace)) as (?) "(Hta & Ht & Hth)".
-  set heapG := HeapG _ _ _ _ _. specialize (HI heapG) as (HIa & HIwp & HIφ).
-  iMod (HIa with "[$Ht $Hth]") as "#HI".
+  iDestruct (inv_alloc N _ (∃ t, trace_half_frag t ∗ ⌜I t⌝) with "[Hth]") as ">#HI".
+  { iNext. eauto. }
   iModIntro. iExists
     (λ σ κs _, (gen_heap_ctx σ.(heap) ∗ trace_auth σ.(trace) ∗ proph_map_ctx κs σ.(used_proph_id))%I),
     (λ _, True%I).
-  iFrame. iSplitL. by iApply HIwp.
+  iFrame. iSplitL.
+  { iDestruct (Hwp (HeapG _ _ _ _ _)) as "Hwp". iApply ("Hwp" with "HI Ht"). }
   iIntros "(_ & Hta & _)". iExists _.
-  iInv "HI" as "Ht'" "_". iDestruct (HIφ with "Hta Ht'") as %?. eauto.
+  iInv "HI" as ">Ht'" "_". iDestruct "Ht'" as (t') "(Ht' & %)".
+  iDestruct (trace_auth_half_frag_agree with "Hta Ht'") as %->. iModIntro. eauto.
 Qed.
 
-(* Require Import iris.program_logic.hoare. *)
+Require Import iris.program_logic.hoare.
 
-(* Lemma module_invariance {Σ} `{heapPreG Σ} (N: namespace) *)
-(*   (Φ: ∀ `{heapG Σ}, iProp Σ → val → iProp Σ)  (* Module specification *) *)
-(*   (P0: iProp Σ) (* Initial resources required by the module *) *)
-(*   (e: val → expr) (* Context program, parameterized by the module *) *)
-(*   (e_init: expr) (* Initialization code, used to allocate resources for P0 *) *)
-(*   (imimpl: val) (* Implementation of the module (instrumented) *) *)
-(*   (good_trace: list val → Prop) (* Trace property *) *)
-(*   (σ: state) (* Initial state *) *)
-(* : *)
-(*   (* The initial trace must satisfy the property *) *)
-(*   good_trace (trace σ) → *)
-(*   (* The context must be safe, given a module satisfying the specification Φ *) *)
-(*   (⊢ ∀ `{heapG Σ} P m, Φ P m -∗ {{{ P }}} e m {{{ v, RET v; True }}}) → *)
-(*   (* The initialization code must provide P0 *) *)
-(*   (⊢ ∀ `{heapG Σ}, {{ True }} e_init {{ _, P0 }}) → *)
-(*   (* The implementation provided for the module (iops) must satisfy the specification Φ. *)
-(*      On top of P0 it is given SL resources for the trace. *) *)
-(*   (⊢ ∀ `{heapG Σ}, Φ (P0 ∗ trace_is (trace σ) ∗ trace_inv N good_trace)%I imimpl) → *)
-(*   (* Then the trace remains good at every step *) *)
-(*   ∀ σ' e', *)
-(*     rtc erased_step ([(e_init;; e imimpl)%E], σ) (e', σ') → *)
-(*     good_trace (trace σ'). *)
-(* Proof. *)
-(*   intros Htrσ Hctx Hinit Himpl σ' e' Hsteps. *)
-(*   eapply heap_invariance. done. by apply Htrσ. 2: eapply Hsteps. *)
-(*   iIntros (?) "HI Htr". wp_bind e_init. *)
-(*   iApply wp_wand. by iApply Hinit. *)
-(*   iIntros (v) "H0". wp_pures. *)
-(*   iApply (Hctx with "[] [H0 Htr HI]"). *)
-(*   - iApply Himpl. *)
-(*   - iFrame. *)
-(*   - eauto. *)
-(* Qed. *)
+Lemma module_invariance {Σ} `{heapPreG Σ} (N: namespace)
+  (Φ: ∀ `{heapG Σ}, iProp Σ → val → iProp Σ)  (* Module specification *)
+  (P0: iProp Σ) (* Initial resources required by the module *)
+  (e: val → expr) (* Context program, parameterized by the module *)
+  (e_init: expr) (* Initialization code, used to allocate resources for P0 *)
+  (imimpl: val) (* Implementation of the module (instrumented) *)
+  (good_trace: list val → Prop) (* Trace property *)
+  (σ: state) (* Initial state *)
+:
+  (* The initial trace must satisfy the property *)
+  good_trace (trace σ) →
+  (* The context must be safe, given a module satisfying the specification Φ *)
+  (⊢ ∀ `{heapG Σ} P m, Φ P m -∗ {{{ P }}} e m {{{ v, RET v; True }}}) →
+  (* The initialization code must provide P0 *)
+  (⊢ ∀ `{heapG Σ}, {{ True }} e_init {{ _, P0 }}) →
+  (* The implementation provided for the module (iops) must satisfy the specification Φ.
+     On top of P0 it is given SL resources for the trace. *)
+  (⊢ ∀ `{heapG Σ}, Φ (P0 ∗ trace_is (trace σ) ∗ trace_inv N good_trace)%I imimpl) →
+  (* Then the trace remains good at every step *)
+  ∀ σ' e',
+    rtc erased_step ([(e_init;; e imimpl)%E], σ) (e', σ') →
+    good_trace (trace σ').
+Proof.
+  intros Htrσ Hctx Hinit Himpl σ' e' Hsteps.
+  eapply heap_invariance. done. by apply Htrσ. 2: eapply Hsteps.
+  iIntros (?) "HI Htr". wp_bind e_init.
+  iApply wp_wand. by iApply Hinit.
+  iIntros (v) "H0". wp_pures.
+  iApply (Hctx with "[] [H0 Htr HI]").
+  - iApply Himpl.
+  - iFrame.
+  - eauto.
+Qed.
+
